% ------------------------------------------------------------------------------
% Problem 2
% ------------------------------------------------------------------------------

Let $p_1$ and $p_2$ be primes, $p_1 < p_2$. Consider
\[ \frac{n^{p_2}}{p_2} + \frac{n^{p_1}}{p_1} + \frac{(p_1 p_2 - p_1 - p_2)n}{p_1 p_2} \]

    First notice
    \[ \frac{n^{p_2}}{p_2} + \frac{n^{p_1}}{p_1} + \frac{(p_1 p_2 - p_1 -
    p_2)n}{p_1 p_2} 
    = 
    \frac
    {p_1 n^{p_2} + p_2 n^{p_1} + p_1 p_2 n - p_1 n - p_2 n}
    {p_1 p_2}
    \]
    
    This expression is an integer if and only if 
    \[p_1 n^{p_2} + p_2 n^{p_1} + p_1 p_2 n - p_1 n - p_2 n \equiv 0 \pmod{p_1 p_2} \]
    
    Using Fermat's Little Theorem, we see that
    \[ n^{p_2} \equiv n \pmod{p_2} \implies  p_1 n^{p_2} \equiv p_1 n  \pmod{p_2} \]
    and 
    \[ n^{p_1} \equiv n \pmod{p_1} \implies  p_2 n^{p_1} \equiv p_2 n \pmod{p_1} \]

\begin{claim}
    \[p_1 n^{p_2} + p_2 n^{p_1} + p_1 p_2 n - p_1 n - p_2 n \equiv 0 \pmod{p_1} \]
\end{claim}
\begin{proof}
    \begin{align*}
    p_1 n^{p_2} + p_2 n^{p_1} + p_1 p_2 n - p_1 n - p_2 n
    &\equiv (0) + (p_2 n) + p_1 p_2 n - p_1 n - p_2 n  \pmod{p_1}\\
    &\equiv p_1 p_2 n - p_1 n \pmod{p_1}\\
    &\equiv p_1 (p_2 -1) n \pmod{p_1}\\
    &\equiv 0 \pmod{p_1}
    \end{align*}
\end{proof}

\begin{claim}
    \[p_1 n^{p_2} + p_2 n^{p_1} + p_1 p_2 n - p_1 n - p_2 n \equiv 0 \pmod{p_2} \]
\end{claim}
\begin{proof}

\end{proof}