\RequirePackage[l2tabu, orthodox]{nag}

\documentclass[letterpaper, 12pt, oneside]{memoir}
\usepackage{amsmath,amsthm,amssymb,mathtools}

% Memoir configuration
\pagestyle{plain}
\setlength{\parindent}{0cm}
\setlength{\parskip}{1ex}

% ------------------------------------------------------------------------------
% Theorem Commands
% ------------------------------------------------------------------------------
\newtheoremstyle{mystyle}% name
    {2ex}       % Space above
    {4ex}       % Space below
    {}          % Body font
    {}          % Indent amount (empty = no indent, \parindent = para indent)
    {\bfseries} % Thm head font
    {.}         % Punctuation after thm head
    {\newline}  % Space after thm head: \newline = linebreak
    {}          % Thm head spec

\theoremstyle{mystyle}
\newtheorem*{prop}{Proposition}
\newtheorem*{lemma}{Lemma}

% ------------------------------------------------------------------------------
% Begin Document
% ------------------------------------------------------------------------------
\title{Math 435 - Homework 1}
\author{George Lamperis}
\date{}

\begin{document}
\maketitle

% ------------------------------------------------------------------------------
% 2.1(a), page 18
% ------------------------------------------------------------------------------
\section*{2.1.(a)}

\begin{lemma}
    If $a$ is an integer, then either $a^2 \equiv 0 \pmod 3$ or 
    $a^2 \equiv 1 \pmod 3$.
\end{lemma}
\begin{proof}
    We have two cases: the case where 3 divides $a$, and the case where 3 does
    not divide $a$.

    If 3 divides $a$, then $a \equiv 0 \pmod 3$. It follows that 
    $a^2 \equiv 0 \pmod 3$ and so we are done.
    
    If 3 does not divide $a$, then either $a \equiv 1 \pmod 3$ or 
    $a \equiv 2 \pmod 3$. Since $2^2 \equiv 1 \pmod 3$, in either case we have
    that $a^2 \equiv 1 \pmod 3$.
\end{proof}


\begin{prop}
    If $(a,b,c)$ is a primitive Pythagorean triple, then either $a$ or $b$ must
    be a multiple of 3.
\end{prop}

\begin{proof}
    If 3 divides $a$ and $b$, then 3 divides $c$. But $a,b,c$ are coprime and
    so we have a contradiction. Hence, it cannot be the case that 3 divides $a$
    and $b$.
    
    Now suppose that $3$ does not divide $a$ or $b$. Then
    $a^2 \equiv 1 \pmod 3$ and $b^2 \equiv 1 \pmod 3$. Since $a^2+b^2 = c^2$, 
    we have that $c^2 \equiv 2 \pmod 3$. But the previous lemma says that this 
    is impossible, and so we have a contradiction.
    
    It follows that exactly one of $a,b$ is divisible by 3.
\end{proof}


% ------------------------------------------------------------------------------
% 2.2, page 19
% ------------------------------------------------------------------------------
\section*{2.2}

\begin{prop}
    Let $m,n, d$ be integers. If an $d$ divides both $m$ and $n$, then $d$ also
    divides $m-n$ and $m+n$.
\end{prop}

\begin{proof}
    Since $d \mid m$, there is an integer $k$ such that $m = dk$. Similarly,
    since $d \mid n$, there is an integer $l$ such that $n = dl$.
    
    Then $m+n = dk+dl = d(k+l)$. Hence $d \mid (m+n)$.
    
    Similarly, $m-n = dk-dl = d(k-l)$. Hence $d \mid (m-n)$.
\end{proof}


% ------------------------------------------------------------------------------
% 2.6, page 19
% ------------------------------------------------------------------------------
\section*{2.6}

\subsection*{2.6.(a)}
\begin{itemize}
  \item $a=99$, $b=20$, $c=101$
  \item $a=143$, $b=24$, $c=145$
\end{itemize}

\subsection*{2.6.(b)}
    $a=1023$, $b=64$, $c=1025$
    
\subsection*{2.6.(c)}
\begin{align*}
    a^2 + b^2 = (a+2)^2 &\implies b^2 = 4a + 4  \\
                    &\implies b = 2 \sqrt{a+1}
\end{align*}

Now let $x = \sqrt{a+1}$. We have
\begin{align*}
    a &= x^2 - 1 \\
    b &= 2x \\
    c &= x^2 + 1   
\end{align*}

Since a is odd, $x$ must be even. Then $(a,b,c)$ will be a primitive Pythagorean
triple for all positive values of $x$.

% ------------------------------------------------------------------------------
% 3.1, page 23
% ------------------------------------------------------------------------------
\section*{3.1}

\subsection*{3.1.(a)}
Suppose $\gcd(u,v) = d$ such that $d > 1$. Then we can write $u = dx$ and 
$v = dy$.

So:
\begin{align*}
    a &= u^2 - v^2          & b &= 2uv          & c &= u^2 + v^2\\
      &= d^2 x^2 - d^2 y^2  &   &= 2(dx)(dy)    &   &= d^2 x^2 + d^2 y^2\\
      &= d^2(x^2 - y^2)     &   &= d^2 (2xy)    &   &= d^2 (x^2 + y^2) \\
\end{align*}

Since $d^2 > 1$ divides $a$, $b$, and $c$, then $(a,b,c)$ is not a primitive
Pythagorean triple.

\subsection*{3.1.(b)}
If $u = 5$ and $v = 1$, $u$ and $v$ are coprime but $(24, 10, 26)$ is not 
primitive because all three values are even.

\subsection*{3.1.(c)}
Below is a table with all values of $u$ and $v$ when we substitute all values
of ${1 \leq v < u \leq 10}$.

\begin{table}[h!]
    \tiny
    \centering
\begin{tabular}{|l l l|l l l l|}
    \hline
    $u$ & $v$ & $\gcd (u, v)$  & $a$   & $b$   & $c$ & $\gcd(a,b,c)$  \\
    \hline
    2 & 1 & 1 & 3 & 4 & 5 & 1 \\
    3 & 1 & 1 & 8 & 6 & 10 & 2 \\
    3 & 2 & 1 & 5 & 12 & 13 & 1 \\
    4 & 1 & 1 & 15 & 8 & 17 & 1 \\
    4 & 2 & 2 & 12 & 16 & 20 & 4 \\
    4 & 3 & 1 & 7 & 24 & 25 & 1 \\
    5 & 1 & 1 & 24 & 10 & 26 & 2 \\
    5 & 2 & 1 & 21 & 20 & 29 & 1 \\
    5 & 3 & 1 & 16 & 30 & 34 & 2 \\
    5 & 4 & 1 & 9 & 40 & 41 & 1 \\
    6 & 1 & 1 & 35 & 12 & 37 & 1 \\
    6 & 2 & 2 & 32 & 24 & 40 & 8 \\
    6 & 3 & 3 & 27 & 36 & 45 & 9 \\
    6 & 4 & 2 & 20 & 48 & 52 & 4 \\
    6 & 5 & 1 & 11 & 60 & 61 & 1 \\
    7 & 1 & 1 & 48 & 14 & 50 & 2 \\
    7 & 2 & 1 & 45 & 28 & 53 & 1 \\
    7 & 3 & 1 & 40 & 42 & 58 & 2 \\
    7 & 4 & 1 & 33 & 56 & 65 & 1 \\
    7 & 5 & 1 & 24 & 70 & 74 & 2 \\
    7 & 6 & 1 & 13 & 84 & 85 & 1 \\
    8 & 1 & 1 & 63 & 16 & 65 & 1 \\
    8 & 2 & 2 & 60 & 32 & 68 & 4 \\
    8 & 3 & 1 & 55 & 48 & 73 & 1 \\
    8 & 4 & 4 & 48 & 64 & 80 & 16 \\
    8 & 5 & 1 & 39 & 80 & 89 & 1 \\
    8 & 6 & 2 & 28 & 96 & 100 & 4 \\
    8 & 7 & 1 & 15 & 112 & 113 & 1 \\
    9 & 1 & 1 & 80 & 18 & 82 & 2 \\
    9 & 2 & 1 & 77 & 36 & 85 & 1 \\
    9 & 3 & 3 & 72 & 54 & 90 & 18 \\
    9 & 4 & 1 & 65 & 72 & 97 & 1 \\
    9 & 5 & 1 & 56 & 90 & 106 & 2 \\
    9 & 6 & 3 & 45 & 108 & 117 & 9 \\
    9 & 7 & 1 & 32 & 126 & 130 & 2 \\
    9 & 8 & 1 & 17 & 144 & 145 & 1 \\
    10 & 1 & 1 & 99 & 20 & 101 & 1 \\
    10 & 2 & 2 & 96 & 40 & 104 & 8 \\
    10 & 3 & 1 & 91 & 60 & 109 & 1 \\
    10 & 4 & 2 & 84 & 80 & 116 & 4 \\
    10 & 5 & 5 & 75 & 100 & 125 & 25 \\
    10 & 6 & 2 & 64 & 120 & 136 & 8 \\
    10 & 7 & 1 & 51 & 140 & 149 & 1 \\
    10 & 8 & 2 & 36 & 160 & 164 & 4 \\
    10 & 9 & 1 & 19 & 180 & 181 & 1 \\
    \hline
\end{tabular}
\end{table}


\subsection*{3.1.(d,e)}
\begin{prop}
    If $u$ and $v$ are coprime and $u-v$ is odd and positive, then $(u^2-v^2,
    2uv, u^2+v^2)$ is a primitive Pythagorean triple.
\end{prop}

\begin{proof}
    Since $u-v$ is odd, exactly one of $u,v$ is odd and the other is even. Then 
    it follows that $u^2-v^2$ and $u^2+v^2$ are odd.

    Suppose $u^2-v^2$ and $2uv$ have a common divisor $d \neq 1$. Since
    $u^2-v^2$ is odd, $d$ must be odd too. Also, since $d \mid 2uv$, either
    $d \mid u$ or $d \mid v$. Let's assume that $d \mid u$.

    Then:
    \begin{align*}
    d \mid 2uv \text{ and } d \mid u^2+v^2  &\implies d \mid u^2+v^2 + 2uv & \\
                                            &\implies d \mid (u+v)^2 \\
                                            &\implies d \mid u+v \\
    \end{align*}

    If $d$ divides $u$ and $u+v$, then there exists $m,n$ such that $dm = u$ and
    $dn = u+v$. Then:
    \begin{align*}
    dn = u+v    &\implies dn = dm+v \\
                &\implies dn-dm = v \\
                &\implies d(n-m) = v \\
    \end{align*}

    So $d \mid v$. But we assumed that $u$ and $v$ were coprime. Then it must
    be the case that $d=1$.

    Hence, $u^2-v^2$, $2uv$, and  $u^2+v^2$ are coprime.
\end{proof}

\end{document}
