\documentclass[12pt, letterpaper]{article}
 
\usepackage[margin=1in]{geometry} 
\usepackage{amsmath,amsthm,amssymb}
\usepackage{enumitem}

\newcommand{\N}{\mathbb{N}}
\newcommand{\Z}{\mathbb{Z}}

\theoremstyle{definition} % disables italics in theorems

\newtheorem{theorem}{Theorem} % master theorem
\newtheorem{lemma}[theorem]{Lemma}
\newtheorem{problem}[theorem]{}

% ------------------------------------------------------------------------------
% Document Begins Here!
%-------------------------------------------------------------------------------
\begin{document}

\title{Math 313 - Problem Set 1}%replace X with the appropriate number
\author{George Lamperis - UIN:664714097} %if necessary, replace with your course title
\date{}
 
\maketitle

% ------------------------------------------------------------------------------
%
% ------------------------------------------------------------------------------

\begin{problem}
    Prove the following identities for elements $x,y,z,w$ of a field:

    \begin{enumerate}[label={\bfseries{(\alph{*})}}]
        \item $(xy)(zw)=(xz)(yw)$.
            \begin{proof}
            \begin{align*}
                (xy)(zw) & = x \cdot (y \cdot (zw))  & \text{ (F6)} \\
                         & = x \cdot ((zw) \cdot y)  & \text{ (F5)} \\
                         & = x \cdot (z \cdot (wy))  & \text{ (F6)} \\
                         & = (xz)(wy)                & \text{ (F6)} \\
                         & = (xz)(yw)                & \text{ (F5)}
            \end{align*}    
            \end{proof}

        \item $(x+y)(z+w) = xz+xw+yz+yw$.
            \begin{proof}
            \begin{align*}
                (x+y)(z+w) & = (x+y) \cdot z + (x+y) \cdot w  &\text{ (F9)} \\
                           & = z \cdot (x+y) + w \cdot (x+y)  &\text{ (F5)} \\
                           & = (zx + zy) + (wx + wy)          &\text{ (F9)} \\
                           & = zx + zy + wz + wy              &\text{ (F2)} \\
                           & = xz + yz + xw + yw              &\text{ (F5)} \\
                           & = xz + xw + yz + yw              &\text{ (F1)}   
            \end{align*}
            \end{proof}

        \item $(-1)x = -x$.
            \begin{proof}
                 We have the identify $0x = 0$.
            \begin{align*}
                0x &= 0 \\
                (1 + (-1))x & = 0  &\text{(F4)}\\
                (1 \cdot x) + ((-1)\cdot x) & = 0  &\text{(F9)} \\
                x + ((-1) \cdot x) & = 0           &\text{(F7)}  
            \end{align*}

                And so by (F4), $x+((-1) \cdot x) = 0  \implies -x = (-1) \cdot$
            \end{proof}
    \end{enumerate}
\end{problem}


\end{document}
