\documentclass[12pt]{article}

\usepackage{amsmath, amsthm, amssymb,amscd}
\usepackage{setspace}
\usepackage{enumerate}
\usepackage{hyperref}
\usepackage[margin=1in]{geometry}



\newtheoremstyle{mystyle}% name
    {2ex}       % Space above
    {2ex}       % Space below
    {}          % Body font
    {}          % Indent amount (empty = no indent, \parindent = para indent)
    {\bfseries} % Thm head font
    {.}         % Punctuation after thm head
    {\newline}  % Space after thm head: \newline = linebreak
    {}          % Thm head spec

\theoremstyle{mystyle}

\newtheorem{thm}{Theorem}
\newtheorem{defn}[thm]{Definition}
\newtheorem{prop}[thm]{Proposition}
\newtheorem{remark}[thm]{Remark}
\newtheorem{example}[thm]{Example}
%\doublespace

% Number sets
\newcommand{\N}{\mathbb{N}}
\newcommand{\Z}{\mathbb{Z}}
\newcommand{\Q}{\mathbb{Q}}
\newcommand{\R}{\mathbb{R}}
\newcommand{\C}{\mathbb{C}}

% ------------------------------------------------------------------------------
% Begin Document
% ------------------------------------------------------------------------------
\title{Math 300 - Final Paper}
\author{George Lamperis}
\date{}

\begin{document}
\maketitle

\section{Introduction}
The number $e$ is extremely important to mathematics. It's called Euler's number
or Napier's number. The number $e$ is intimately related to the logarithm.

The number $e$ was discovered through the study of logarithms. The motivation
for the development of logarithms was an attempt to make multiplication easier
by turning it into addition instead. In 1618, John Napier release an essay which
is considered to be the first work on logarithms. In this essay appears a table
of logarithms to the base $e$. However, Napier was unaware of the number $e$
and it's connection to logarithms.

In 1683, Jacob Bernoulli was studying compound interest. He tried to find the
limit of $(1 + 1/n)^n$ as $n$ tends to infinity. Although this limit is equal to
$e$, Bernoulli likely did not realize the connection between $e$ and the
logarithm.

A Swiss mathematican named Leonhard Euler, after whom the number $e$ is named.
Euler discovered many remarkable properties of the number $e$.



\section{Results}

\begin{defn}
  Define the function $L: (0, \infty) \mapsto \R$ as follows:
  $$ L(x) = \int_1^x \frac{dt}{t} $$
  
  The function $x \mapsto 1/x$ is continuous. Therefore, by the Fundamental
  Theorem of Calculus, $L$ is differentiable and
  $$ L^\prime(x) = \frac{1}{x} $$.
  
  Notice also that
  $$L(1) = 0$$
  
  Since $L'(x) > 0$ for all $x \in (0, \R)$,  we can deduce that $L(x)$ is
  strictly monotone increasing on its entire domain \cite[Theorem 4.13]{howie}.
  
  Additionally, since $L(x)$ is monotone increasing, we can apply the Integral
  Test, \cite[Theorem 5.37]{howie}. Since the series $\sum_1^n \frac{1}{x}$
  diverges, it follows that $L(x)$ diverges also.
\end{defn}


\begin{thm}
  For all $x,y \in (0, \infty)$,
  $$ L(xy) = L(x) + L(y) \text{ and } L(1/x) = -L(x)$$
\end{thm}
\begin{proof}
  This proof borrows heavily from \cite[Theorem 6.1]{howie}
  \begin{align*}
    L(xy) &= \int_{1}^{xy} \frac{dt}{t} \\
          &= \int_{1}^{x} \frac{dt}{t} + \int_{x}^{xy} \frac{dt}{t} \\
          &= L(x) + \int_{x}^{xy} \frac{dt}{t}
  \end{align*}
  Now in the remaining integral, substitute $u = t/x$. 
  \begin{align*}
          &= L(x) + \int_{1}^{y} \frac{du}{u} \\
          &= L(x) + L(y)
  \end{align*}
  as desired.
  
  The next property follows immediately from this:
  \begin{align*}
    L(x) + L(1/x) &= L(x \cdot 1/x) \\
                  &= L(1) \\
                  &= 0
  \end{align*}  

\end{proof}


\begin{thm}
  There is a unique number $e$ such that 
  $$ L(e) = \int_1^e \frac{dt}{t} = 1 $$
\end{thm}
\begin{proof}
  We know that $L(1) = 0$. Additionally, because $L(x)$ diverges, there is a $c$
  such that $L(c) > 1$. Now, apply the Intermediate Value Theorem and we have
  that there exists a number $e$, such that $1 < e < c$, and $L(x) = 1$. Because
  $L(x)$ is strictly monotone increasing, and thus bijective, it follows that
  $e$ is unique.
\end{proof}


\begin{defn}
  Since $L$ is differentiable and monotone increasing, there is a monotone
  increasing and differentiable inverse fuction $L^{-1}: \R \mapsto (0, \infty)$,
  which we will denote by $E$. And so we have
  \begin{align*}
    E(L(X)) = x \\
    L(E(x)) = x
  \end{align*}
  
  Note also that
  $$ E(0) = 1 \text{ and } E(1) = e $$
\end{defn}


\begin{thm}
  The function $E$ is its own derivative, i.e., $E^\prime(x) = E(x)$
\end{thm}
\begin{proof}
  This proof is taken from \cite[p. 168]{howie}:
  \begin{align*}
    E^\prime(x) 
        &= \frac{1}{L^\prime(L^{-1}(x))}  & \text{(Howie, Theorem 4.15)} \\
        &= L^\prime(x) \\
        &= E(x)
  \end{align*}
\end{proof}


\begin{thm}
  For all $x,y \in \R$, we have
  $$ E(x+y) = E(x)E(y) $$
  and
  $$ E(-x) = \frac{1}{E(x)}$$
\end{thm}
\begin{proof}
  This proof is taken from \cite[Theorem 6.2]{howie}
  Let $x,y \in \R$. Then
  \begin{align*}
    E(x+y) &= E[L(E(x)) + L(E(y))] \\
           &= E[L(E(x)E(y))] \\
           &= E(x)E(y)
  \end{align*}
  
  The second property follows since
  $$ E(x)E(-x) = E(x +(-x)) = E(0) = 1 $$
\end{proof}


From the previous theorem, we can deduce that
  $$E(x)^2 = E(x)E(x) = E(x+x) = E(2x)$$
or more generally, for a real number $n$,
  $$ E(x)^n = E(nx)$$.

Now let us gather this information and introduce a new notation.

\begin{thm}
  Define $e^x$ as $E(x)$ and also define $\log_e (y)$ (or equivalently $\ln y$)
  as $L(y)$.
  
  Now let us express what we know about $L$ and $E$ using this new notation.
  Recall that $E$ and $L$ are inverses. Thus,
  $$ e^{\ln x} = x \text{ and } \ln(e^x) = x $$
  
  We also have the following properties:
  \begin{align*}
    \int_{1}^x \frac{dt}{t} = \ln x \\
    \frac{d}{dx}(\ln x) = \frac{1}{x} \\
    \ln xy = \ln x + \ln y \\
    \ln(1/x) = - \ln x \\
    \frac{d}{dx}(e^x) = e^x \\
  \end{align*}
\end{thm}


Before this result, the function $a^x$ is only defined for rational numbers. The
following result defines $a^x$ for any real number $x$.
\begin{defn}
  If $a$ is a positive real number, we define $a^x$ as
  $$ a^x = e^{x \ln a} $$
  and
  $$ \log_a x = \frac{\ln x}{\ln a} $$
\end{defn}


\begin{thm}
  If $b > 0$ and $\frac{d}{dx} b^x = b^x$, then $b = e$.
\end{thm}
\begin{proof}
  \begin{align*}
    (b^x)' &= (e^{x \ln b})^\prime \\
           &= (e^{x \ln b}) \cdot (x \ln b)^\prime  \\
           &= b^x \cdot \ln b
  \end{align*}
  
  Hence, it must the case that $\ln b = 1$. Since $e$ is the unique number such
  that $\ln e = 1$, it follows that $b=e$.
\end{proof}


\begin{remark}
  If we apply the Taylor-Maclaurin Theorem to $e^x$, we have
  \begin{align*}
    e^x &= e^0 + xe^0 + \frac{x^2}{2!}e^0 + \frac{x^3}{3!} +  \ldots \\
        &= \sum_1^\infty \frac{x^n}{n!}
  \end{align*}
\end{remark}

\begin{thm}
  The number $e$ is irrational. 
\end{thm}
\begin{proof}
  This proof is taken from \cite[Example 6.10]{howie}
  Suppose for contradiction that $e = p/q$ for integers $p,q$. Let $n$ be an
  integer such that $n > max(q,3)$. It follows that $n!e$ is an integer. Now
  apply Taylor's Theorem:
  $$ e = 2 + \frac{1}{2!} + \ldots + \frac{1}{n!} + \frac{1}{(n+1)!}e^\theta $$
  where $0 < \theta < 1$. Hence
  $$ \frac{e^\theta}{n+1} = n!e - 2n! - \frac{n!}{2!} - \ldots - \frac{n!}{n!} $$
  is an integer. On the other hand, $1 < e^\theta < 3$, and so 
  $$ 0< \frac{e^\theta}{n_1} < \frac{3}{n+1} < 1 $$
  and so we have a contradiction. Therefore, we deduce that $e$ is irrational.
  
\end{proof}



\section{Practical uses}

\begin{example}
  Recall that when we apply the Taylor-Maclaurin Theorem to $e^x$, we have
  $$ e^x = \sum_1^\infty \frac{x^n}{n!} $$
  
  Because this series converges extremely fast, it provides us with an accurate
  way to approximate the value of $e$. In fact, Euler used this series to give
  the approximation.
\end{example}


\begin{example}
  Here is a clever trick used to make multiplication of large numbers easier.
  This was commonly used by physicists and engineers before calculators and
  computers were available. 
  \begin{align*}
    xy &= e^{\ln xy} \\
       &= e^{\ln x + \ln y} \\
  \end{align*}
  This is particularly useful when $x$ and $y$ are very large numbers.
  Calculating their product using the typical method for multiplying is quite
  tedious. But using this trick, you look up $\ln x$ and $\ln y$ in a log table.

  Scientific notation really helps.
   
\end{example}

% Maybe include some old-fashioned tricks for evaluating numbers with logs.

% ------------------------------------------------------------------------------
% References
% ------------------------------------------------------------------------------
\begin{thebibliography}{10}

\bibitem{howie}
John M. Howie, Real Analysis

\bibitem{proofwiki1}
\url{http://www.proofwiki.org/wiki/Derivative_of_Natural_Logarithm_Function/Proof_2}

\bibitem{SWAU}
\url{http://turner.faculty.swau.edu/mathematics/math110de/materials/logtable/}
\end{thebibliography}


\end{document}